Launchbury/Arity-Nominal.thy
@@ -2,6 +2,10 @@ theory "Arity-Nominal"
 imports Arity "Nominal-HOLCF"
 begin
 
+lemma join_eqvt[eqvt]: "\<pi> \<bullet> (x \<squnion> (y :: 'a :: {Finite_Join_cpo, cont_pt})) = (\<pi> \<bullet> x) \<squnion> (\<pi> \<bullet> y)"
+  by (rule is_joinI[symmetric]) (auto simp add: perm_below_to_right)
+
+
 instantiation Arity :: pure
 begin
   definition "p \<bullet> (a::Arity) = a"
