Launchbury/ArityAnalysis.thy
@@ -27,6 +27,4 @@ lemma Aexp'_eqvt[eqvt]: "\<pi> \<bullet> (ArityAnalysis.Aexp' Aexp e) = ArityAna
   unfolding ArityAnalysis.Aexp'_def
   by perm_simp rule
 
-
-
 end
