Launchbury/ArityCorrect.thy
@@ -15,18 +15,17 @@ begin
     with Aexp_edom have "v \<notin> edom (Aexp e\<cdot>a)" by auto
     thus ?thesis unfolding edom_def by simp
   qed
-  
 
 end
 
 locale SubstArityAnalysis = EdomArityAnalysis + 
-  assumes Aexp_subst: "Aexp (e[y::=x])\<cdot>a \<sqsubseteq> env_delete y ((Aexp e)\<cdot>a) \<squnion> AE_singleton x\<cdot>(up\<cdot>0)"
+  assumes Aexp_subst: "Aexp (e[y::=x])\<cdot>a \<sqsubseteq> env_delete y ((Aexp e)\<cdot>a) \<squnion> esing x\<cdot>(up\<cdot>0)"
   assumes Aexp_subst_restr: "x \<notin> S \<Longrightarrow> y \<notin> S \<Longrightarrow> (Aexp e[x::=y] \<cdot> a) f|` S = (Aexp e\<cdot>a) f|` S"
 
 locale CorrectArityAnalysis' = SubstArityAnalysis +
 (*  assumes Aexp_eqvt: "\<pi> \<bullet> Aexp = Aexp" *)
   assumes Aexp_Var: "up \<cdot> n \<sqsubseteq> (Aexp (Var x)\<cdot>n) x"
-  assumes Aexp_App: "Aexp e \<cdot>(inc\<cdot>n) \<squnion> AE_singleton x \<cdot> (up\<cdot>0) \<sqsubseteq>  Aexp (App e x) \<cdot> n"
+  assumes Aexp_App: "Aexp e \<cdot>(inc\<cdot>n) \<squnion> esing x \<cdot> (up\<cdot>0) \<sqsubseteq>  Aexp (App e x) \<cdot> n"
   assumes Aexp_Lam: "env_delete y (Aexp e \<cdot>(pred\<cdot>n)) \<sqsubseteq> Aexp (Lam [y]. e) \<cdot> n"
 
 locale CorrectArityAnalysisAheap' = CorrectArityAnalysis' + 
@@ -50,10 +49,10 @@ end
 context CorrectArityAnalysis'
 begin
 
-lemma Aexp_Var_singleton: "AE_singleton x \<cdot> (up\<cdot>n) \<sqsubseteq> Aexp (Var x) \<cdot> n"
+lemma Aexp_Var_singleton: "esing x \<cdot> (up\<cdot>n) \<sqsubseteq> Aexp (Var x) \<cdot> n"
   by (simp add: Aexp_Var)
 
-lemma Aexp'_Var: "AE_singleton x \<cdot> n \<sqsubseteq> Aexp' (Var x) \<cdot> n"
+lemma Aexp'_Var: "esing x \<cdot> n \<sqsubseteq> Aexp' (Var x) \<cdot> n"
   by (cases n) (simp_all add: Aexp_Var)
 
 end
