Launchbury/CoCallAnalysis.thy
@@ -5,6 +5,7 @@ begin
 locale CoCallAnalysis =
   fixes ccExp :: "exp \<Rightarrow> Arity \<rightarrow> CoCalls"
 begin
+
 definition ccExp' :: "exp \<Rightarrow> Arity\<^sub>\<bottom> \<rightarrow> CoCalls"
   where "ccExp' e = fup \<cdot> (ccExp e)"
 
@@ -38,5 +39,6 @@ locale CorrectCoCallAnalysis = CoCallAnalysis_ccField +
   assumes Aexp_Lam1: "ccExp (Lam [y]. e) \<cdot> (inc\<cdot>n) = cc_delete y (ccExp e \<cdot>n)"
   assumes Aexp_App: "ccExp (App e x)\<cdot>n = ccExp e \<cdot>(inc\<cdot>n) \<squnion> ccProd (fv e) {x}"
   (* assumes Aexp_subst_restr: "x \<notin> S \<Longrightarrow> y \<notin> S \<Longrightarrow> (ccExp e[x::=y] \<cdot> a) f|` S = (ccExp e\<cdot>a) f|` S" *)
+
 
 end
