Launchbury/CoCallCardinality.thy
@@ -1,764 +1,6 @@
 theory CoCallCardinality
-imports FTreeCardinality CoCallAnalysis
+imports FTreeCardinality CoCallAnalysis "CoCallGraph-FTree"
 begin
-
-lemma subset_ccNeighbors:
-  "S \<subseteq> ccNeighbors {x} G \<longleftrightarrow> ccProd {x} S \<sqsubseteq> G"
-  by transfer (auto simp add: sym_def)
-
-lemma elem_ccNeighbors:
-  "xa \<in> ccNeighbors {x} G \<longleftrightarrow> (xa--x\<in>G)"
-  by transfer (auto simp add: sym_def)
-
-lemma cont_edom[THEN cont_compose, simp, cont2cont]:
-  "cont (\<lambda> f. edom f)"
-  apply (rule set_contI)
-  apply (auto simp add: edom_def)
-  apply (metis ch2ch_fun lub_eq_bottom_iff lub_fun)
-  apply (metis ch2ch_fun lub_eq_bottom_iff lub_fun)
-  done
-
-(*
-definition ccApprox :: "var ftree \<Rightarrow> CoCalls"
-  where "ccApprox t =  lub (ccFromList ` (paths t))"
-*)
-lift_definition ccApprox :: "var ftree \<Rightarrow> CoCalls"
-  is "\<lambda> xss .  lub (ccFromList ` xss)".
-
-lemma ccApprox_paths: "ccApprox t = lub (ccFromList ` (paths t))" by transfer simp
-
-lemma ccApprox_strict[simp]: "ccApprox \<bottom> = \<bottom>"
-  by (simp add: ccApprox_paths empty_is_bottom[symmetric])
-
-lemma in_ccApprox: "(x--y\<in>(ccApprox t)) \<longleftrightarrow> (\<exists> xs \<in> paths t. (x--y\<in>(ccFromList xs)))"
-  unfolding ccApprox_paths
-  by transfer auto
-
-lemma ccApprox_mono: "paths t \<subseteq> paths t' \<Longrightarrow> ccApprox t \<sqsubseteq> ccApprox t'"
-  by (rule below_CoCallsI) (auto simp add: in_ccApprox)
-
-lemma ccApprox_mono': "t \<sqsubseteq>  t' \<Longrightarrow> ccApprox t \<sqsubseteq> ccApprox t'"
-  by (metis below_set_def ccApprox_mono paths_mono_iff)
-
-lemma ccApprox_belowI: "(\<And> xs. xs \<in> paths t \<Longrightarrow> ccFromList xs \<sqsubseteq> G) \<Longrightarrow> ccApprox t \<sqsubseteq> G"
-  unfolding ccApprox_paths
-  by transfer auto
-
-lemma ccApprox_below_iff: "ccApprox t \<sqsubseteq> G \<longleftrightarrow> (\<forall> xs \<in> paths t. ccFromList xs \<sqsubseteq> G)"
-  unfolding ccApprox_paths by transfer auto
-
-lemma cc_restr_ccApprox_below_iff: "cc_restr S (ccApprox t) \<sqsubseteq> G \<longleftrightarrow> (\<forall> xs \<in> paths t. cc_restr S (ccFromList xs) \<sqsubseteq> G)"
-  unfolding ccApprox_paths cc_restr_lub
-  by transfer auto
-
-lemma ccFromList_below_ccApprox:
-  "xs \<in> paths t \<Longrightarrow> ccFromList xs \<sqsubseteq> ccApprox t" 
-by (rule below_CoCallsI)(auto simp add: in_ccApprox)
-
-lemma ccApprox_nxt_below:
-  "ccApprox (nxt t x) \<sqsubseteq> ccApprox t"
-by (rule below_CoCallsI)(auto simp add: in_ccApprox paths_nxt_eq elim!:  bexI[rotated])
-
-lemma ccFromList_filter[simp]: "x--y\<in>ccFromList (filter P xs) \<longleftrightarrow> x--y\<in>ccFromList xs \<and> P x \<and> P y"
-  by (induction xs) auto
-
-lemma ccApprox_ftree_restr_nxt_below:
-  "ccApprox (ftree_restr S (nxt t x)) \<sqsubseteq> ccApprox (ftree_restr S t)"
-by (rule below_CoCallsI)
-   (auto simp add: in_ccApprox filter_paths_conv_free_restr[symmetric] paths_nxt_eq  elim!:  bexI[rotated])
-
-lemma ccApprox_ftree_restr[simp]: "ccApprox (ftree_restr S t) = cc_restr S (ccApprox t)"
-  by (rule CoCalls_eqI) (auto simp add: in_ccApprox filter_paths_conv_free_restr[symmetric] )
-
-lemma interleave_ccFromList:
-  "xs \<in> interleave ys zs \<Longrightarrow> ccFromList xs = ccFromList ys \<squnion> ccFromList zs \<squnion> ccProd (set ys) (set zs)"
-  by (induction rule: interleave_induct)
-     (auto simp add: interleave_set ccProd_comm ccProd_insert2[where S' = "set xs" for xs]  ccProd_insert1[where S' = "set xs" for xs] )
-
-lemma ccApprox_both: "ccApprox (t \<otimes>\<otimes> t') = ccApprox t \<squnion> ccApprox t' \<squnion> ccProd (carrier t) (carrier t')"
-proof (rule below_antisym)
-  show "ccApprox (t \<otimes>\<otimes> t') \<sqsubseteq> ccApprox t \<squnion> ccApprox t' \<squnion> ccProd (carrier t) (carrier t')"
-  by (rule below_CoCallsI)
-     (auto 4 4  simp add: in_ccApprox paths_both Union_paths_carrier[symmetric]  interleave_ccFromList)
-next
-  have "ccApprox t \<sqsubseteq> ccApprox (t \<otimes>\<otimes> t')"
-    by (rule ccApprox_mono[OF both_contains_arg1])
-  moreover
-  have "ccApprox t' \<sqsubseteq> ccApprox (t \<otimes>\<otimes> t')"
-    by (rule ccApprox_mono[OF both_contains_arg2])
-  moreover
-  have "ccProd (carrier t) (carrier t') \<sqsubseteq> ccApprox (t \<otimes>\<otimes> t')"
-  proof(rule ccProd_belowI)
-    fix x y
-    assume "x \<in> carrier t" and "y \<in> carrier t'"
-    then obtain xs ys where "x \<in> set xs" and "y \<in> set ys"
-      and "xs \<in> paths t" and "ys \<in> paths t'" by (auto simp add: Union_paths_carrier[symmetric])
-    hence "xs @ ys \<in> paths (t \<otimes>\<otimes> t')" by (metis paths_both append_interleave)
-    moreover
-    from `x \<in> set xs` `y \<in> set ys`
-    have "x--y\<in>(ccFromList (xs@ys))" by simp
-    ultimately
-    show "x--y\<in>(ccApprox (t \<otimes>\<otimes> t'))" by (auto simp add: in_ccApprox simp del: ccFromList_append)
-  qed
-  ultimately
-  show "ccApprox t \<squnion> ccApprox t' \<squnion> ccProd (carrier t) (carrier t') \<sqsubseteq> ccApprox (t \<otimes>\<otimes> t')"
-    by (simp add: join_below_iff)
-qed
-
-lemma wild_recursion:
-  assumes "ccApprox  t \<sqsubseteq> G"
-  assumes "\<And> x. x \<notin> S \<Longrightarrow> f x = empty"
-  assumes "\<And> x. x \<in> S \<Longrightarrow> ccApprox (f x) \<sqsubseteq> G"
-  assumes "\<And> x. x \<in> S \<Longrightarrow> ccProd (ccNeighbors S G) (carrier (f x)) \<sqsubseteq> G"
-  shows "ccApprox (ftree_restr (-S) (substitute f {} t)) \<sqsubseteq> G"
-proof(rule ccApprox_belowI)
-  fix xs
-
-  def seen \<equiv> "{} :: var set"
-
-  assume "xs \<in> paths (ftree_restr (- S) (substitute f {} t))"
-  then obtain xs' xs'' T where "xs = [x\<leftarrow>xs' . x \<notin> S]" and "substitute'' f T xs'' xs'" and "T = {}" and "xs'' \<in> paths t"
-    by (auto simp add: filter_paths_conv_free_restr2[symmetric] substitute_substitute'')
- 
-  note this(2,3)
-  moreover
-  from `ccApprox t \<sqsubseteq> G` and `xs'' \<in> paths t`
-  have  "ccFromList xs'' \<sqsubseteq> G"
-    by (auto simp add: ccApprox_below_iff)
-  moreover
-  note assms(2)
-  moreover
-  from assms(3-4)
-  have "\<And> x ys. x \<in> S \<Longrightarrow> ys \<in> paths (f x) \<Longrightarrow> ccFromList ys \<sqsubseteq> G"
-    and "\<And> x ys. x \<in> S \<Longrightarrow> ys \<in> paths (f x) \<Longrightarrow> ccProd (ccNeighbors S G) (set ys) \<sqsubseteq> G"
-    by (auto simp add: ccApprox_below_iff Union_paths_carrier[symmetric] cc_lub_below_iff)
-  moreover
-  have "ccProd seen (set xs'') \<sqsubseteq> G" unfolding seen_def by simp
-  ultimately 
-  have "ccFromList [x\<leftarrow>xs' . x \<notin> S] \<sqsubseteq> G \<and> ccProd seen (set xs') \<sqsubseteq> G"
-  proof(induction f T xs'' xs' arbitrary: seen rule: substitute''.induct[case_names Nil Cons])
-  case Nil thus ?case by simp
-  next
-  case (Cons zs f x xs' xs T ys)
-    from `T = {}` have [simp]: "f_nxt f T x = f" by (simp add: f_nxt_def)
-
-    have seen_x: "ccProd seen {x} \<sqsubseteq> G"
-      using Cons.prems
-      by (auto simp add: ccProd_insert2[where S' = "set xs" for xs] join_below_iff)
-
-    show ?case
-    proof(cases "x \<in> S")
-      case True
-
-      from Cons.prems
-      have "ccProd {x} (set xs) \<sqsubseteq> G" by (auto simp add: join_below_iff)
-      with `x \<in> S`
-      have subset1: "set xs \<subseteq> ccNeighbors S G" by transfer auto
-
-      from Cons.prems
-      have "seen \<subseteq> ccNeighbors {x} G"
-        by (auto simp add: subset_ccNeighbors ccProd_insert2[where S' = "set xs" for xs] join_below_iff ccProd_comm)
-      hence subset2: "seen \<subseteq> ccNeighbors S G" 
-        by (rule order_trans[OF _ ccNeighbors_mono[OF insert_subsetI[OF  `x \<in> S`  empty_subsetI] below_refl]])
-        
-      from True Cons.prems Cons.hyps
-      have "ccFromList [x\<leftarrow>ys . x \<notin> S] \<sqsubseteq> G \<and> ccProd seen (set ys) \<sqsubseteq> G"
-        apply -
-        apply (rule Cons.IH)
-        apply (auto simp add: ccApprox_both join_below_iff ftree_restr_both interleave_ccFromList interleave_set  ccProd_insert2[where S' = "set xs" for xs]
-                   intro: below_trans[OF ccProd_mono1[OF subset1]]  below_trans[OF ccProd_mono1[OF subset2]])
-        done
-      with True seen_x
-      show "ccFromList [x\<leftarrow>x # ys . x \<notin> S] \<sqsubseteq> G  \<and> ccProd seen (set (x#ys)) \<sqsubseteq> G" 
-        by (auto simp add: ccProd_insert2[where S' = "set xs" for xs] join_below_iff)
-    next
-      case False
-  
-      from False Cons.prems Cons.hyps
-      have "ccFromList [x\<leftarrow>ys . x \<notin> S] \<sqsubseteq> G \<and> ccProd (insert x seen) (set ys) \<sqsubseteq> G"
-        apply -
-        apply (rule Cons.IH[where seen = "insert x seen"])
-        apply (auto simp add: ccApprox_both join_below_iff ftree_restr_both interleave_ccFromList
-                   simp add:  ccProd_insert2[where S' = "set xs" for xs]
-                   simp add:  ccProd_insert1[where S' = "seen"])
-        done
-      moreover
-      from this
-      have "ccProd {x} (set ys) \<sqsubseteq>  G"
-        by (auto simp add: ccProd_insert1[where S' = "seen"] join_below_iff)
-      hence "ccProd {x} {x \<in> set ys. x \<notin> S} \<sqsubseteq> G"
-        by (rule below_trans[rotated, OF _ ccProd_mono2]) auto
-      moreover
-      note False seen_x
-      ultimately
-      show "ccFromList [x\<leftarrow>x # ys . x \<notin> S] \<sqsubseteq> G \<and> ccProd seen (set (x # ys)) \<sqsubseteq> G"
-        by (auto simp add: join_below_iff  simp add:  ccProd_insert2[where S' = "set xs" for xs]   ccProd_insert1[where S' = "seen"])
-    qed
-  qed
-  with `xs = _`
-  show "ccFromList xs \<sqsubseteq> G" by simp
-qed
-
-lemma ccFromList_replicate[simp]: "ccFromList (replicate n x) = (if n \<le> 1 then \<bottom>  else ccProd {x} {x})"
-  by (induction n) auto
-
-lemma ccApprox_many_calls[simp]:
-  "ccApprox (many_calls x) = ccProd {x} {x}"
-  by transfer' (rule CoCalls_eqI, auto)
-
-lemma ccApprox_single[simp]:
-  "ccApprox (FTree.single y) = \<bottom>"
-  by transfer' auto
-
-lemma carrier_single[simp]: "carrier (single y) = {y}"
-  by transfer auto
-
-lemma ccApprox_either[simp]: "ccApprox (t \<oplus>\<oplus> t') = ccApprox t \<squnion> ccApprox t'"
-  by transfer' (rule CoCalls_eqI, auto)
-
-
-inductive_set valid_lists :: "var set \<Rightarrow> CoCalls \<Rightarrow> var list set"
-  for S G
-  where  "[] \<in> valid_lists S G"
-  | "set xs \<subseteq> ccNeighbors {x} G \<Longrightarrow> xs \<in> valid_lists S G \<Longrightarrow> x \<in> S \<Longrightarrow> x#xs \<in> valid_lists S G"
-
-inductive_simps valid_lists_simps[simp]: "[] \<in> valid_lists S G" "(x#xs) \<in> valid_lists S G"
-inductive_cases vald_lists_ConsE: "(x#xs) \<in> valid_lists S G"
-
-lemma  valid_lists_downset_aux:
-  "xs \<in> valid_lists S CoCalls \<Longrightarrow> butlast xs \<in> valid_lists S CoCalls"
-  by (induction xs) (auto dest: in_set_butlastD)
-
-lift_definition ccFTree :: "var set \<Rightarrow> CoCalls \<Rightarrow> var ftree" is "\<lambda> S G. valid_lists S G" 
-  by (auto intro: valid_lists_downset_aux)
-
-lemma valid_lists_subset: "xs \<in> valid_lists S G \<Longrightarrow> set xs \<subseteq> S"
-  by (induction rule: valid_lists.induct) auto
-
-lemma paths_ccFTree[simp]: "paths (ccFTree S G) = valid_lists S G" by transfer auto
-
-
-lemma carrier_ccFTree[simp]: "carrier (ccFTree S G) = S"
-  apply transfer
-  apply (auto dest: valid_lists_subset)
-  apply (rule_tac x = "[x]" in bexI)
-  apply auto
-  done
-
-lemma ccProd_below_cc_restr:
-  "ccProd S S' \<sqsubseteq> cc_restr S'' G \<longleftrightarrow> ccProd S S' \<sqsubseteq> G \<and> (S = {} \<or> S' = {} \<or> S \<subseteq> S'' \<and> S' \<subseteq> S'')"
-  by transfer auto
-
-lemma valid_lists_ccFromList:
-  "xs \<in> valid_lists S G \<Longrightarrow> ccFromList xs \<sqsubseteq> cc_restr S G"
-by (induction rule:valid_lists.induct)
-   (auto simp add: join_below_iff subset_ccNeighbors ccProd_below_cc_restr elim: set_mp[OF valid_lists_subset])
-
-lemma ccApprox_ccFTree[simp]: "ccApprox (ccFTree S G) = cc_restr S G"
-proof (transfer' fixing: S G, rule below_antisym)
-  show "lub (ccFromList ` valid_lists S G) \<sqsubseteq> cc_restr S G"
-    apply (rule is_lub_thelub_ex)
-    apply (metis coCallsLub_is_lub)
-    apply (rule is_ubI)
-    apply clarify
-    apply (erule valid_lists_ccFromList)
-    done
-next
-  show "cc_restr S G \<sqsubseteq> lub (ccFromList ` valid_lists S G)"
-  proof (rule below_CoCallsI)
-    fix x y
-    have "x--y\<in>(ccFromList [y,x])" by simp
-    moreover
-    assume "x--y\<in>(cc_restr S G)"
-    hence "[y,x] \<in> valid_lists S G"  by (auto simp add: elem_ccNeighbors)
-    ultimately
-    show "x--y\<in>(lub (ccFromList ` valid_lists S G))"
-      by (rule in_CoCallsLubI[OF _ imageI])
-  qed
-qed
-
-lemma below_ccFTreeI:
-  assumes "carrier t \<subseteq> S" and "ccApprox t \<sqsubseteq> G"
-  shows "t \<sqsubseteq> ccFTree S G"
-unfolding paths_mono_iff[symmetric] below_set_def
-proof
-  fix xs
-  assume "xs \<in> paths t"
-  with assms
-  have "xs \<in> valid_lists S G"
-  proof(induction xs arbitrary : t)
-  case Nil thus ?case by simp
-  next
-  case (Cons x xs)
-    from `x # xs \<in> paths t`
-    have "possible t x" and "xs \<in> paths (nxt t x)" by (auto simp add: Cons_path)
-
-    have "ccProd {x} (set xs) \<sqsubseteq> ccFromList (x # xs)" by simp
-    also
-    from `x # xs \<in> paths t` 
-    have "\<dots> \<sqsubseteq> ccApprox t"
-      by (rule ccFromList_below_ccApprox)
-    also
-    note `ccApprox t \<sqsubseteq> G`
-    finally
-    have "ccProd {x} (set xs) \<sqsubseteq> G" by this simp_all
-    hence "set xs \<subseteq> ccNeighbors {x} G" unfolding subset_ccNeighbors.
-    moreover
-    have "xs \<in> valid_lists S G"
-    proof(rule Cons.IH)
-      show "xs \<in> paths (nxt t x)" by fact
-    next
-      from `carrier t \<subseteq> S`
-      show "carrier (nxt t x) \<subseteq> S" 
-        by (rule order_trans[OF carrier_nxt_subset])
-    next
-      from `ccApprox t \<sqsubseteq> G`
-      show "ccApprox (nxt t x) \<sqsubseteq> G" 
-        by (rule below_trans[OF ccApprox_nxt_below])
-    qed
-    moreover
-    from  `carrier t \<subseteq> S` and `possible t x`
-    have "x \<in> S" by (rule carrier_possible_subset)
-    ultimately
-    show ?case..
-  qed
-    
-  thus "xs \<in> paths (ccFTree S G)" by (metis paths_ccFTree)
-qed    
-
-lemma mono_ccFTree1:
-  "S \<subseteq> S' \<Longrightarrow> ccFTree S G \<sqsubseteq> ccFTree S' G"
-  by (rule below_ccFTreeI) (auto simp add:  cc_restr_below_arg)
-
-lemma valid_lists_chain1:
-   assumes "chain Y" 
-   assumes "xs \<in> valid_lists (UNION UNIV Y) G"
-   shows "\<exists> i. xs \<in> valid_lists (Y i) G"
-proof-
-  note `chain Y`
-  moreover
-  from assms(2)
-  have "set xs \<subseteq> UNION UNIV Y" by (rule valid_lists_subset)
-  moreover
-  have "finite (set xs)" by simp
-  ultimately
-  have "\<exists>i. set xs \<subseteq> Y i" by (rule finite_subset_chain)
-  then obtain i where "set xs \<subseteq> Y i"..
-
-  from assms(2) this
-  have "xs \<in> valid_lists (Y i) G" by (induction rule:valid_lists.induct) auto
-  thus ?thesis..
-qed
-
-lemma valid_lists_chain2:
-   assumes "chain Y" 
-   assumes "xs \<in> valid_lists S (\<Squnion>i. Y i)"
-   shows "\<exists> i. xs \<in> valid_lists S  (Y i)"
-using assms(2)
-proof(induction rule:valid_lists.induct[case_names Nil Cons])
-  case Nil thus ?case by simp
-next
-  case (Cons xs x)
-
-  from `chain Y`
-  have "chain (\<lambda> i. ccNeighbors {x} (Y i))"
-    apply (intro chainI)
-    unfolding below_set_def
-    by (intro ccNeighbors_mono order_refl chainE)
-  moreover
-  from `set xs \<subseteq> ccNeighbors {x} (\<Squnion> i. Y i)`
-  have "set xs \<subseteq> (\<Union> i. ccNeighbors {x} (Y i))"
-    by (simp add:  lub_set)
-  moreover
-  have "finite (set xs)" by simp
-  ultimately
-  have "\<exists>i. set xs \<subseteq> ccNeighbors {x} (Y i)" by (rule finite_subset_chain)
-  then obtain i where i: "set xs \<subseteq> ccNeighbors {x} (Y i)"..
-
-  from Cons.IH
-  obtain j where j: "xs \<in> valid_lists S (Y j)"..
-
-  from i
-  have "set xs \<subseteq> ccNeighbors {x} (Y (max i j))"
-    by (rule order_trans[OF _ ccNeighbors_mono[OF order_refl chain_mono[OF `chain Y` max.cobounded1]]])
-  moreover
-  from j
-  have "xs \<in> valid_lists S (Y (max i j))" 
-    by (induction rule: valid_lists.induct)
-       (auto del: subsetI elim: order_trans[OF _ ccNeighbors_mono[OF order_refl chain_mono[OF `chain Y` max.cobounded2]]])
-  moreover
-  note `x \<in> S`
-  ultimately
-  have "x # xs \<in> valid_lists S (Y (max i j))" by rule
-  thus ?case..
-qed
-
-lemma cont_ccFTree1:
-  "cont (\<lambda> S. ccFTree S G)"
-  apply (rule contI2)
-  apply (rule monofunI)
-  apply (erule mono_ccFTree1[folded below_set_def])
-  
-  apply (rule ftree_belowI)
-  apply (simp add: paths_Either lub_set lub_is_either)
-  apply (drule (1) valid_lists_chain1[rotated])
-  apply simp
-  done
-
-lemma cFTree_mono2:
-  "G \<sqsubseteq> G' \<Longrightarrow> ccFTree S G \<sqsubseteq> ccFTree S G'"
-  apply (rule ftree_belowI)
-  apply simp
-  apply (induct_tac  rule:valid_lists.induct) apply assumption
-  apply simp
-  apply simp
-  apply (erule (1) order_trans[OF _ ccNeighbors_mono[OF order_refl]])
-  done
-
-lemma cont_ccFTree2:
-  "cont (ccFTree S)"
-  apply (rule contI2)
-  apply (rule monofunI)
-  apply (erule cFTree_mono2)
-
-  apply (rule ftree_belowI)
-  apply (simp add: paths_Either lub_set lub_is_either)
-  apply (drule (1) valid_lists_chain2)
-  apply simp
-  done
-
-
-lemmas cont_ccFTree = cont_compose2[where c = ccFTree, OF cont_ccFTree1 cont_ccFTree2, simp, cont2cont]
-
-
-
-lemma ccFTree_below_singleI:
-  assumes "S \<inter> S' \<inter> ccManyCalls G = {}"
-  shows "ccFTree S G \<sqsubseteq> singles S'"
-proof-
-  {
-  fix xs x
-  assume "x \<in> S'"
-
-  assume "xs \<in> valid_lists S G"
-  hence "length [x'\<leftarrow>xs . x' = x] \<le> Suc 0"
-  proof(induction rule: valid_lists.induct[case_names Nil Cons])
-    case Nil thus ?case by simp
-  next
-    case (Cons xs x')
-    show ?case
-    proof(cases "x' = x")
-      case True with `x' \<in> S`
-      have "x \<in> S" by simp
-      from this `x \<in> S'`
-      have "x--x\<notin>G" using assms by auto
-      hence "x \<notin> ccNeighbors {x} G" by (metis elem_ccNeighbors)
-      with Cons
-      show ?thesis by (auto simp add: filter_empty_conv)
-    next
-      case False
-      with Cons
-      show ?thesis by auto
-    qed
-  qed
-  }
-  thus ?thesis by transfer auto
-qed
-
-lemma valid_lists_mono1:
-  assumes "S \<subseteq> S'"
-  shows "valid_lists S G \<subseteq> valid_lists S' G"
-proof
-  fix xs
-  assume "xs \<in> valid_lists S G"
-  thus "xs \<in> valid_lists S' G"
-    by (induction rule: valid_lists.induct) (auto dest: set_mp[OF assms])
-qed
-
-
-lemma ccFTree_mono1: "S \<subseteq> S' \<Longrightarrow> ccFTree S G \<sqsubseteq> ccFTree S' G"
-  by transfer (rule valid_lists_mono1)
-
-lemma ccFTree_mono2: "G \<sqsubseteq> G' \<Longrightarrow> ccFTree S G \<sqsubseteq> ccFTree S G'"
-  by (rule cont2monofunE[OF cont_ccFTree2])
-
-lemma valid_lists_cc_restr: "valid_lists S G = valid_lists S (cc_restr S G)"
-proof(rule set_eqI)
-  fix xs
-  show "(xs \<in> valid_lists S G) = (xs \<in> valid_lists S (cc_restr S G))"
-    by (induction xs) (auto dest: set_mp[OF valid_lists_subset])
-qed
-
-lemma ccFTree_cc_restr: "ccFTree S G = ccFTree S (cc_restr S G)"
-  by transfer' (rule valid_lists_cc_restr)
-
-lemma ccFTree_cong_below: "cc_restr S G \<sqsubseteq> cc_restr S G' \<Longrightarrow> ccFTree S G \<sqsubseteq> ccFTree S G'"
-  by (metis ccFTree_mono2 ccFTree_cc_restr)
-  
-lemma ccFTree_cong: "cc_restr S G = cc_restr S G' \<Longrightarrow> ccFTree S G = ccFTree S G'"
-  by (metis ccFTree_cc_restr)
-
-lemma interleave_valid_list:
-  "xs \<in> ys \<otimes> zs \<Longrightarrow> ys \<in> valid_lists S G \<Longrightarrow> zs \<in> valid_lists S' G' \<Longrightarrow> xs \<in> valid_lists (S \<union> S') (G \<squnion> (G' \<squnion> ccProd S S'))"
-proof (induction rule:interleave_induct)
-  case Nil
-  show ?case by simp
-next
-  case (left ys zs xs x)
-
-  from `x # ys \<in> valid_lists S G`
-  have "x \<in> S" and "set ys \<subseteq> ccNeighbors {x} G" and "ys \<in> valid_lists S G"
-    by auto
- 
-  from `xs \<in> ys \<otimes> zs`
-  have "set xs = set ys \<union> set zs" by (rule interleave_set)
-  with `set ys \<subseteq> ccNeighbors {x} G` valid_lists_subset[OF `zs \<in> valid_lists S' G'`]
-  have "set xs \<subseteq> ccNeighbors {x} (G \<squnion> (G' \<squnion> ccProd S S'))"
-    by (auto simp add: ccNeighbors_ccProd `x \<in> S`)
-  moreover
-  from `ys \<in> valid_lists S G` `zs \<in> valid_lists S' G'`
-  have "xs \<in> valid_lists (S \<union> S') (G \<squnion> (G' \<squnion> ccProd S S'))"
-    by (rule left.IH)
-  moreover
-  from `x \<in> S`
-  have "x \<in> S \<union> S'" by simp
-  ultimately
-  show ?case..
-next
-  case (right ys zs xs x)
-
-  from `x # zs \<in> valid_lists S' G'`
-  have "x \<in> S'" and "set zs \<subseteq> ccNeighbors {x} G'" and "zs \<in> valid_lists S' G'"
-    by auto
- 
-  from `xs \<in> ys \<otimes> zs`
-  have "set xs = set ys \<union> set zs" by (rule interleave_set)
-  with `set zs \<subseteq> ccNeighbors {x} G'` valid_lists_subset[OF `ys \<in> valid_lists S G`]
-  have "set xs \<subseteq> ccNeighbors {x} (G \<squnion> (G' \<squnion> ccProd S S'))"
-    by (auto simp add: ccNeighbors_ccProd `x \<in> S'`)
-  moreover
-  from `ys \<in> valid_lists S G` `zs \<in> valid_lists S' G'`
-  have "xs \<in> valid_lists (S \<union> S') (G \<squnion> (G' \<squnion> ccProd S S'))"
-    by (rule right.IH)
-  moreover
-  from `x \<in> S'`
-  have "x \<in> S \<union> S'" by simp
-  ultimately
-  show ?case..
-qed
-
-lemma interleave_ccFTree: 
-   "ccFTree S G \<otimes>\<otimes> ccFTree S' G' \<sqsubseteq> ccFTree (S \<union> S') (G \<squnion> G' \<squnion> ccProd S S')"
-   by transfer' (auto, erule (2) interleave_valid_list)
-
-lemma interleave_valid_list':
-  "xs \<in> valid_lists (S \<union> S') G \<Longrightarrow> \<exists> ys zs. xs \<in> ys \<otimes> zs \<and> ys \<in> valid_lists S G \<and> zs \<in> valid_lists S' G"
-proof(induction rule: valid_lists.induct[case_names Nil Cons])
-  case Nil show ?case by simp
-next
-  case (Cons xs x)
-  then obtain ys zs where "xs \<in> ys \<otimes> zs" "ys \<in> valid_lists S G" "zs \<in> valid_lists S' G" by auto
-
-    from `xs \<in> ys \<otimes> zs` have "set xs = set ys \<union> set zs" by (rule interleave_set)
-    with `set xs \<subseteq> ccNeighbors {x} G` 
-    have "set ys \<subseteq> ccNeighbors {x} G" and "set zs \<subseteq> ccNeighbors {x} G"  by auto
-  
-  from `x \<in> S \<union> S'`
-  show ?case
-  proof
-    assume "x \<in> S"
-    with `set ys \<subseteq> ccNeighbors {x} G` `ys \<in> valid_lists S G`
-    have "x # ys \<in> valid_lists S G"
-      by rule
-    moreover
-    from `xs \<in> ys \<otimes> zs`
-    have "x#xs \<in> x#ys \<otimes> zs"..
-    ultimately
-    show ?thesis using `zs \<in> valid_lists S' G` by blast
-  next
-    assume "x \<in> S'"
-    with `set zs \<subseteq> ccNeighbors {x} G` `zs \<in> valid_lists S' G`
-    have "x # zs \<in> valid_lists S' G"
-      by rule
-    moreover
-    from `xs \<in> ys \<otimes> zs`
-    have "x#xs \<in> ys \<otimes> x#zs"..
-    ultimately
-    show ?thesis using `ys \<in> valid_lists S G` by blast
-  qed
-qed
-
-
-lemma interleave_ccFTree': 
-   "ccFTree (S \<union> S') G \<sqsubseteq> ccFTree S G \<otimes>\<otimes> ccFTree S' G"
-   by transfer' (auto dest!:  interleave_valid_list')
-
-
-lemma many_calls_valid_list:
-  "xs \<in> valid_lists {x} (ccProd {x} {x}) \<Longrightarrow> xs \<in> range (\<lambda>n. replicate n x)"
-  by (induction rule: valid_lists.induct) (auto, metis UNIV_I image_iff replicate_Suc)
-
-lemma many_calls_ccFTree:
-  shows "many_calls x = ccFTree {x} (ccProd {x} {x})"
-  apply(transfer')
-  apply (auto intro: many_calls_valid_list)
-  apply (induct_tac n)
-  apply (auto simp add: ccNeighbors_ccProd)
-  done
-
-lemma filter_valid_lists:
-  "xs \<in> valid_lists S G \<Longrightarrow> filter P xs \<in> valid_lists {a \<in> S. P a} G"
-by (induction rule:valid_lists.induct) auto
-
-lemma filter_valid_lists':
-  "xs \<in> valid_lists {x' \<in> S. P x'} G \<Longrightarrow> xs \<in> filter P ` valid_lists S G"
-proof (induction xs )
-  case Nil thus ?case by auto  (metis filter.simps(1) image_iff valid_lists_simps(1))
-next
-  case (Cons x xs)
-  from Cons.prems
-  have "set xs \<subseteq> ccNeighbors {x} G" and "xs \<in> valid_lists {x' \<in> S. P x'} G" and "x \<in> S" and "P x" by auto
-
-  from this(2) have "set xs \<subseteq> {x' \<in> S. P x'}" by (rule valid_lists_subset)
-  hence "\<forall>x \<in> set xs. P x" by auto
-  hence [simp]: "filter P xs = xs" by (rule filter_True)
-  
-  from Cons.IH[OF `xs \<in> _`]
-  have "xs \<in> filter P ` valid_lists S G".
-
-  from  `xs \<in> valid_lists {x' \<in> S. P x'} G`
-  have "xs \<in> valid_lists S G" by (rule set_mp[OF valid_lists_mono1, rotated]) auto
-
-  from `set xs \<subseteq> ccNeighbors {x} G` this `x \<in> S`
-  have "x # xs \<in> valid_lists S G" by rule
-
-  hence "filter P (x # xs) \<in> filter P ` valid_lists S G" by (rule imageI)
-  thus ?case using `P x` `filter P xs =xs` by simp
-qed
-
-lemma without_ccFTree[simp]:
-   "without x (ccFTree S G) = ccFTree (S - {x}) G"
-by (transfer' fixing: x) (auto dest: filter_valid_lists'  filter_valid_lists[where P = "(\<lambda> x'. x'\<noteq> x)"]  simp add: set_diff_eq)
-
-lemma repeatable_ccFTree_ccSquare: "S \<subseteq> S' \<Longrightarrow> repeatable (ccFTree S (ccSquare S'))"
-   unfolding repeatable_def
-   by transfer (auto simp add:ccNeighbors_ccSquare dest: set_mp[OF valid_lists_subset])
-
-lemma multi_calls_ccFTree:
-  assumes "xs \<in> paths (ccFTree S G)"
-  assumes "\<not> one_call_in_path x xs"
-  shows "x \<in> S" and "x \<in> ccManyCalls G"
-proof-
-  from assms(1) have "xs \<in> valid_lists S G" by simp 
-
-  have "x \<in> set xs" by (metis assms(2) filter_True one_call_in_path_filter)
-  with `xs \<in> valid_lists S G`
-  show "x \<in> S" by (metis  subsetCE valid_lists_subset)
-
-  show "x \<in> ccManyCalls G"
-  proof(rule ccontr)
-    assume "x \<notin> ccManyCalls G"
-    with `xs \<in> valid_lists S G` 
-    have "one_call_in_path x xs"
-    by (induction rule: valid_lists.induct) (auto simp add: no_call_in_path_set_conv)
-    with assms(2)
-    show False..
-  qed
-qed
-
-
-text {* An alternative definition *}
-
-inductive valid_lists' :: "var set \<Rightarrow> CoCalls \<Rightarrow> var set \<Rightarrow> var list \<Rightarrow> bool"
-  for S G
-  where  "valid_lists' S G prefix []"
-  | "prefix \<subseteq> ccNeighbors {x} G \<Longrightarrow> valid_lists' S G (insert x prefix) xs \<Longrightarrow> x \<in> S \<Longrightarrow> valid_lists' S G prefix (x#xs)"
-
-inductive_simps valid_lists'_simps[simp]: "valid_lists' S G prefix []" "valid_lists' S G prefix (x#xs)"
-inductive_cases vald_lists'_ConsE: "valid_lists' S G prefix (x#xs)"
-
-lemma valid_lists_valid_lists':
-  "xs \<in> valid_lists S G \<Longrightarrow> ccProd prefix (set xs) \<sqsubseteq> G \<Longrightarrow> valid_lists' S G prefix xs"
-proof(induction arbitrary: prefix rule: valid_lists.induct[case_names Nil Cons])
-  case Nil thus ?case by simp
-next
-  case (Cons xs x)
-
-  from Cons.prems Cons.hyps Cons.IH[where prefix = "insert x prefix"]
-  show ?case
-  by (auto simp add: insert_is_Un[where A = "set xs"]  insert_is_Un[where A = prefix]
-                     join_below_iff subset_ccNeighbors elem_ccNeighbors ccProd_comm simp del: Un_insert_left )
-qed
-
-lemma valid_lists'_valid_lists_aux:
-  "valid_lists' S G prefix xs \<Longrightarrow>  x \<in> prefix \<Longrightarrow> ccProd (set xs) {x} \<sqsubseteq> G"
-proof(induction  rule: valid_lists'.induct[case_names Nil Cons])
-  case Nil thus ?case by simp
-next
-  case (Cons prefix x xs)
-  thus ?case
-    apply (auto simp add: ccProd_insert2[where S' = prefix] ccProd_insert1[where S' = "set xs"] join_below_iff subset_ccNeighbors)
-    by (metis Cons.hyps(1) dual_order.trans empty_subsetI insert_subset subset_ccNeighbors)
-qed
-
-lemma valid_lists'_valid_lists:
-  "valid_lists' S G prefix xs \<Longrightarrow> xs \<in> valid_lists S G"
-proof(induction  rule: valid_lists'.induct[case_names Nil Cons])
-  case Nil thus ?case by simp
-next
-  case (Cons prefix x xs)
-  thus ?case
-    by (auto simp add: insert_is_Un[where A = "set xs"]  insert_is_Un[where A = prefix]
-                   join_below_iff subset_ccNeighbors elem_ccNeighbors ccProd_comm simp del: Un_insert_left 
-         intro: valid_lists'_valid_lists_aux)
-qed
-
-text {* Yet another definition *}
-
-lemma valid_lists_characterization:
-  "xs \<in> valid_lists S G \<longleftrightarrow> set xs \<subseteq> S \<and> (\<forall>n. ccProd (set (take n xs)) (set (drop n xs)) \<sqsubseteq> G)"
-proof(safe)
-  fix x
-  assume "xs \<in> valid_lists S G"
-  from  valid_lists_subset[OF this]
-  show "x \<in> set xs \<Longrightarrow> x \<in> S" by auto
-next
-  fix n
-  assume "xs \<in> valid_lists S G"
-  thus "ccProd (set (take n xs)) (set (drop n xs)) \<sqsubseteq> G"
-  proof(induction arbitrary: n rule: valid_lists.induct[case_names Nil Cons])
-    case Nil thus ?case by simp
-  next
-    case (Cons xs x)
-    show ?case
-    proof(cases n)
-      case 0 thus ?thesis by simp
-    next
-      case (Suc n)
-      with Cons.hyps Cons.IH[where n = n]
-      show ?thesis
-      apply (auto simp add: ccProd_insert1[where S' = "set xs" for xs] join_below_iff subset_ccNeighbors)
-      by (metis dual_order.trans set_drop_subset subset_ccNeighbors)
-    qed
-  qed
-next
-  assume "set xs \<subseteq> S"
-  and "\<forall> n. ccProd (set (take n xs)) (set (drop n xs)) \<sqsubseteq> G" 
-  thus "xs \<in> valid_lists S G"
-  proof (induction xs)
-    case Nil thus ?case by simp
-  next
-    case (Cons x xs)
-    from `\<forall>n. ccProd (set (take n (x # xs))) (set (drop n (x # xs))) \<sqsubseteq> G`
-    have "\<forall>n. ccProd (set (take n xs)) (set (drop n xs)) \<sqsubseteq> G"
-      by -(rule, erule_tac x = "Suc n" in allE, auto simp add: ccProd_insert1[where S' = "set xs" for xs] join_below_iff)
-    from Cons.prems Cons.IH[OF _ this]
-    have "xs \<in> valid_lists S G" by auto
-    with Cons.prems(1)  spec[OF `\<forall>n. ccProd (set (take n (x # xs))) (set (drop n (x # xs))) \<sqsubseteq> G`, where x = 1]
-    show ?case by (simp add: subset_ccNeighbors)
-  qed
-qed
-  
 
 
 locale CoCallCardinality = CoCallAnalysis + CoCallAnalyisHeap + CorrectArityAnalysisLet' +
@@ -767,16 +9,6 @@ locale CoCallCardinality = CoCallAnalysis + CoCallAnalyisHeap + CorrectArityAnal
   assumes ccExp_subst: "x \<notin>  S \<Longrightarrow> y \<notin> S \<Longrightarrow> cc_restr S (ccExp e[y::=x]\<cdot>a) \<sqsubseteq> cc_restr S (ccExp e\<cdot>a)"
   assumes ccExp_pap: "isLam e \<Longrightarrow> ccExp e\<cdot>0 = ccSquare (fv e)"
   assumes ccExp_Let: "cc_restr (-domA \<Gamma>) (ccHeap \<Gamma> e\<cdot>a) \<sqsubseteq> ccExp (Let \<Gamma> e)\<cdot>a"
-  (*
-  assumes ccExp_ccField: "ccField (ccExp e\<cdot>a) \<subseteq> fv e"
-  *)
-
-  (*  assumes ccHeap_ccField: "ccField (ccHeap \<Gamma> e\<cdot>a) \<subseteq> domA \<Gamma>" *)
-  
-  (*
-  assumes linear_Exp: "isLinear \<Delta> e a \<Longrightarrow> ccLinear (domA \<Delta>) (ccExp e\<cdot>a)"
-  assumes linear_Heap: "isLinear \<Delta> e a \<Longrightarrow> map_of \<Delta> x = Some e' \<Longrightarrow> (Aheap \<Delta> e\<cdot>a) x= up\<cdot>a' \<Longrightarrow> ccLinear (domA \<Delta>) (ccExp e'\<cdot>a')"
-  *)
 
   assumes ccHeap_Exp: "ccExp e\<cdot>a \<sqsubseteq> ccHeap \<Delta> e\<cdot>a"
   assumes ccHeap_Heap: "map_of \<Delta> x = Some e' \<Longrightarrow> (Aheap \<Delta> e\<cdot>a) x= up\<cdot>a' \<Longrightarrow> ccExp e'\<cdot>a' \<sqsubseteq> ccHeap \<Delta> e\<cdot>a"
@@ -791,23 +23,22 @@ locale CoCallCardinality = CoCallAnalysis + CoCallAnalyisHeap + CorrectArityAnal
 
 begin
 
-(*
-lemma cc_restr_ccExp': "cc_restr (fv e) (ccExp e\<cdot>a) = ccExp e\<cdot>a"
-  by (rule cc_restr_noop[OF ccExp_ccField])
-*)
-
 definition Fexp :: "exp \<Rightarrow> Arity \<rightarrow> var ftree"
   where "Fexp e = (\<Lambda> a. ccFTree (edom (Aexp e \<cdot>a)) (ccExp e\<cdot>a))"
 
 lemma Fexp_simp: "Fexp e\<cdot>a = ccFTree (edom (Aexp e \<cdot>a)) (ccExp e\<cdot>a)"
-  unfolding Fexp_def
-  by simp
+  unfolding Fexp_def by simp
 
 lemma carrier_Fexp': "carrier (Fexp e\<cdot>a) \<subseteq> fv e"
   unfolding Fexp_simp carrier_ccFTree
   by (rule Aexp_edom)
 
 sublocale FutureAnalysis Fexp.
+
+lemma carrier_AnalBinds_below:
+  "carrier ((Fexp.AnalBinds  \<Delta>\<cdot>(Aheap \<Delta> e\<cdot>a)) x) \<subseteq> edom ((ABinds \<Delta>)\<cdot>(Aheap \<Delta> e\<cdot>a))"
+by (auto simp add: Fexp.AnalBinds_lookup Fexp_def split: option.splits 
+         elim!: set_mp[OF edom_mono[OF monofun_cfun_fun[OF ABind_below_ABinds]]])
 
 sublocale FutureAnalysisCarrier Fexp
   by default (rule carrier_Fexp')
@@ -908,485 +139,11 @@ qed
 definition Fheap :: "heap \<Rightarrow> exp \<Rightarrow> Arity \<rightarrow> var ftree"
   where "Fheap \<Gamma> e = (\<Lambda> a. ftree_restr (edom (Aheap \<Gamma> e\<cdot>a)) anything)"
 
-
-lemma range_filter[simp]: "range (filter P) = {xs. set xs \<subseteq> Collect P}"
-  apply auto
-  apply (rule_tac x = x in rev_image_eqI)
-  apply simp
-  apply (rule sym)
-  apply (auto simp add: filter_id_conv)
-  done
-
-lemma ftree_restr_anything_cont[THEN cont_compose, simp, cont2cont]:
-  "cont (\<lambda> S. ftree_restr S anything)"
-  apply (rule ftree_contI3)
-  apply (rule set_contI)
-  apply (auto simp add: filter_paths_conv_free_restr[symmetric] lub_set)
-  apply (rule finite_subset_chain)
-  apply auto
-  done
-
 lemma Fheap_simp: "Fheap \<Gamma> e\<cdot>a = ftree_restr (edom (Aheap \<Gamma> e\<cdot>a)) anything"
   unfolding Fheap_def by simp
 
 lemma carrier_Fheap':"carrier (Fheap \<Gamma> e\<cdot>a) = edom (Aheap \<Gamma> e\<cdot>a)"
     unfolding Fheap_simp carrier_ccFTree by simp
-
-lemma carrier_substitute_aux:
-  assumes "xs \<in> paths (substitute f T t)"
-  assumes "carrier t \<subseteq> A"
-  assumes "\<And> x. x \<in> A \<Longrightarrow> carrier (f x) \<subseteq> A" 
-  shows   "set xs \<subseteq> A"
-  using assms
-  apply(induction  f T t xs rule: substitute_induct)
-  apply auto
-  apply (metis carrier_possible_subset)
-  apply (metis carrier_f_nxt carrier_nxt_subset carrier_possible_subset contra_subsetD order_trans)
-  done
-
-text {*
-It is tricky to relate @{term substitute} and @{term ccApprox}.
-We do this separately for no-recursive bindings, linearly-recursive bindings and others.
-*}
-
-
-
- 
-lemma ccFromList_filter[simp]:
-  "ccFromList (filter P xs) = cc_restr {x. P x} (ccFromList xs)"
-by (induction xs) (auto simp add: Collect_conj_eq)
-
-lemma cc_restr_Compl_eq[simp]:
-  "cc_restr {x. x \<notin> S} = cc_restr (-S)"
-  by (metis Compl_eq)
-
-
-lemma substitute_not_carrier:
-  assumes "x \<notin> carrier t"
-  assumes "\<And> x'. x \<notin> carrier (f x')"
-  shows "x \<notin>  carrier (substitute f T t)"
-proof-
-  have "ftree_restr ({x}) (substitute f T t) = ftree_restr ({x}) t"
-  proof(rule ftree_rest_substitute)
-    fix x'
-    from `x \<notin> carrier (f x')`
-    show "carrier (f x') \<inter> {x} = {}" by auto
-  qed
-  hence "x \<notin> carrier (ftree_restr ({x}) (substitute f T t)) \<longleftrightarrow> x \<notin> carrier (ftree_restr ({x}) t)" by metis
-  with assms(1)
-  show ?thesis by simp
-qed
-
-
-
-
-lemma both_below_singles1:
-  assumes "t \<sqsubseteq> singles S"
-  assumes "carrier t' \<inter> S = {}"
-  shows "t \<otimes>\<otimes> t' \<sqsubseteq> singles S"
-proof (rule ftree_belowI)
-  fix xs
-  assume "xs \<in> paths (t \<otimes>\<otimes> t')"
-  then obtain ys zs where "ys \<in> paths t" and "zs \<in> paths t'" and "xs \<in> ys \<otimes> zs" by (auto simp add: paths_both)
-  with assms 
-  have "ys \<in> paths (singles S)" and "set zs \<inter> S = {}"
-    by (metis below_ftree.rep_eq contra_subsetD paths.rep_eq, auto simp add: Union_paths_carrier[symmetric])
-  with `xs \<in> ys \<otimes> zs`
-  show "xs \<in> paths (singles S)"
-    by (induction) (auto simp add: paths_singles no_call_in_path_set_conv interleave_set dest: more_than_one_setD split: if_splits)
-qed
-
-lemma substitute_below_singlesI:
-  assumes "t \<sqsubseteq> singles S"
-  assumes "\<And> x. carrier (f x) \<inter> S = {}"
-  shows "substitute f T t \<sqsubseteq> singles S"
-proof(rule ftree_belowI)
-  fix xs
-  assume "xs \<in> paths (substitute f T t)"
-  thus "xs \<in> paths (singles S)"
-  using assms
-  proof(induction f T t xs arbitrary: S rule: substitute_induct)
-    case Nil
-    thus ?case by simp
-  next
-    case (Cons f T t x xs)
-
-    from `x#xs \<in> _`
-    have xs: "xs \<in> paths (substitute (f_nxt f T x) T (nxt t x \<otimes>\<otimes> f x))" by auto
-    moreover
-
-    from `t \<sqsubseteq> singles S`
-    have "nxt t x \<sqsubseteq> singles S" 
-      by (metis "FTree-HOLCF.nxt_mono" below_trans nxt_singles_below_singles)
-    from this `carrier (f x) \<inter> S = {}`
-    have "nxt t x \<otimes>\<otimes> f x \<sqsubseteq> singles S"
-      by (rule both_below_singles1)
-    moreover
-    { fix x'
-      from  `carrier (f x') \<inter> S = {}`
-      have "carrier (f_nxt f T x x') \<inter> S = {}"
-        by (auto simp add: f_nxt_def)
-    }
-    ultimately
-    have IH: "xs \<in> paths (singles S)"
-      by (rule Cons.IH) 
-  
-  show ?case
-    proof(cases "x \<in> S")
-      case True
-      with `carrier (f x) \<inter> S = {}`
-      have "x \<notin> carrier (f x)" by auto
-      moreover
-      from `t \<sqsubseteq> singles S`
-      have "nxt t x \<sqsubseteq> nxt (singles S) x" by (rule nxt_mono)
-      hence "carrier (nxt t x) \<subseteq> carrier (nxt (singles S) x)" by (rule carrier_mono)
-      from set_mp[OF this] True
-      have "x \<notin> carrier (nxt t x)" by auto
-      ultimately
-      have "x \<notin> carrier (nxt t x \<otimes>\<otimes> f x)" by simp
-      hence "x \<notin> carrier (substitute (f_nxt f T x) T (nxt t x \<otimes>\<otimes> f x))"
-      proof(rule substitute_not_carrier)
-        fix x'  
-        from `carrier (f x') \<inter> S = {}` `x \<in> S`
-        show "x \<notin> carrier (f_nxt f T x x')" by (auto simp add: f_nxt_def)
-      qed
-      with xs
-      have "x \<notin> set xs" by (auto simp add: Union_paths_carrier[symmetric])
-      with IH
-      have "xs \<in> paths (without x (singles S))" by (rule paths_withoutI)
-      thus ?thesis using True by (simp add: Cons_path)
-    next
-      case False
-      with IH
-      show ?thesis by (simp add: Cons_path)
-    qed
-  qed
-qed
-
-(*
-lemma linear_recursion:
-  assumes "ccLinear S (ccApprox t)"
-  assumes "ccApprox  t \<sqsubseteq> G"
-  assumes "\<And> x. x \<notin> S \<Longrightarrow> f x = empty"
-  assumes "\<And> x. x \<in> S \<Longrightarrow> ccLinear S (ccApprox (f x))"
-  assumes "\<And> x. x \<in> S \<Longrightarrow> ccApprox (f x) \<sqsubseteq> G"
-  assumes "\<And> x. x \<in> S \<Longrightarrow> ccProd (ccNeighbors S G) (carrier (f x)) \<sqsubseteq> G"
-  shows "ccApprox (ftree_restr (-S) (substitute f {} t)) \<sqsubseteq> G"
-proof(rule ccApprox_belowI)
-  fix xs
-
-  def seen \<equiv> "{} :: var set"
-
-  assume "xs \<in> paths (ftree_restr (- S) (substitute f {} t))"
-  then obtain xs' xs'' T where "xs = [x\<leftarrow>xs' . x \<notin> S]" and "substitute'' f T xs'' xs'" and "T = {}" and "xs'' \<in> paths t"
-    by (auto simp add: filter_paths_conv_free_restr2[symmetric] substitute_substitute'')
- 
-  note this(2,3)
-  moreover
-  from `ccLinear S (ccApprox t)` and `ccApprox t \<sqsubseteq> G` and `xs'' \<in> paths t`
-  have "ccLinear S (ccFromList xs'')" and "ccFromList xs'' \<sqsubseteq> G"
-    by (auto simp add: ccLinear_ccApprox ccApprox_below_iff)
-  moreover
-  note assms(3)
-  moreover
-  from assms(4-6)
-  have "\<And> x ys. x \<in> S \<Longrightarrow> ys \<in> paths (f x) \<Longrightarrow> ccLinear S (ccFromList ys)"
-    and "\<And> x ys. x \<in> S \<Longrightarrow> ys \<in> paths (f x) \<Longrightarrow> ccFromList ys \<sqsubseteq> G"
-    and "\<And> x ys. x \<in> S \<Longrightarrow> ys \<in> paths (f x) \<Longrightarrow> ccProd (ccNeighbors S G) (set ys) \<sqsubseteq> G"
-    by (auto simp add: ccLinear_ccApprox ccApprox_below_iff Union_paths_carrier[symmetric] cc_lub_below_iff)
-  moreover
-  have "ccProd seen (set xs'') \<sqsubseteq> G" unfolding seen_def by simp
-  ultimately 
-  have "ccFromList [x\<leftarrow>xs' . x \<notin> S] \<sqsubseteq> G \<and> ccProd seen (set xs') \<sqsubseteq> G"
-  proof(induction f T xs'' xs' arbitrary: seen rule: substitute''.induct[case_names Nil Cons])
-  case Nil thus ?case by simp
-  next
-  case (Cons zs f x xs' xs T ys)
-    from `T = {}` have [simp]: "f_nxt f T x = f" by (simp add: f_nxt_def)
-
-    have seen_x: "ccProd seen {x} \<sqsubseteq> G"
-      using Cons.prems
-      by (auto simp add: ccProd_insert2[where S' = "set xs" for xs] join_below_iff)
-
-    show ?case
-    proof(cases "x \<in> S")
-      case True
-
-      from Cons.prems
-      have "ccProd {x} (set xs) \<sqsubseteq> G" by (auto simp add: join_below_iff)
-      with `x \<in> S`
-      have subset1: "set xs \<subseteq> ccNeighbors S G" by transfer auto
-
-      from Cons.prems
-      have "seen \<subseteq> ccNeighbors {x} G"
-        by (auto simp add: subset_ccNeighbors ccProd_insert2[where S' = "set xs" for xs] join_below_iff ccProd_comm)
-      hence subset2: "seen \<subseteq> ccNeighbors S G" 
-        by (rule order_trans[OF _ ccNeighbors_mono[OF insert_subsetI[OF  `x \<in> S`  empty_subsetI] below_refl]])
-        
-      from True Cons.prems Cons.hyps
-      have "ccFromList [x\<leftarrow>ys . x \<notin> S] \<sqsubseteq> G \<and> ccProd seen (set ys) \<sqsubseteq> G"
-        apply -
-        apply (rule Cons.IH)
-        apply (auto simp add: ccApprox_both join_below_iff ftree_restr_both interleave_ccFromList interleave_set  ccProd_insert2[where S' = "set xs" for xs]
-                   intro: below_trans[OF ccProd_mono1[OF subset1]]  below_trans[OF ccProd_mono1[OF subset2]])
-        done
-      with True seen_x
-      show "ccFromList [x\<leftarrow>x # ys . x \<notin> S] \<sqsubseteq> G  \<and> ccProd seen (set (x#ys)) \<sqsubseteq> G" 
-        by (auto simp add: ccProd_insert2[where S' = "set xs" for xs] join_below_iff)
-    next
-      case False
-  
-      from False Cons.prems Cons.hyps
-      have "ccFromList [x\<leftarrow>ys . x \<notin> S] \<sqsubseteq> G \<and> ccProd (insert x seen) (set ys) \<sqsubseteq> G"
-        apply -
-        apply (rule Cons.IH[where seen = "insert x seen"])
-        apply (auto simp add: ccApprox_both join_below_iff ftree_restr_both interleave_ccFromList
-                   simp add:  ccProd_insert2[where S' = "set xs" for xs]
-                   simp add:  ccProd_insert1[where S' = "seen"])
-        done
-      moreover
-      from this
-      have "ccProd {x} (set ys) \<sqsubseteq>  G"
-        by (auto simp add: ccProd_insert1[where S' = "seen"] join_below_iff)
-      hence "ccProd {x} {x \<in> set ys. x \<notin> S} \<sqsubseteq> G"
-        by (rule below_trans[rotated, OF _ ccProd_mono2]) auto
-      moreover
-      note False seen_x
-      ultimately
-      show "ccFromList [x\<leftarrow>x # ys . x \<notin> S] \<sqsubseteq> G \<and> ccProd seen (set (x # ys)) \<sqsubseteq> G"
-        by (auto simp add: join_below_iff  simp add:  ccProd_insert2[where S' = "set xs" for xs]   ccProd_insert1[where S' = "seen"])
-    qed
-  qed
-  with `xs = _`
-  show "ccFromList xs \<sqsubseteq> G" by simp
-qed
-*)
-
-(*
-text {*
-It is tricky to relate @{term substitute} and @{term ccApprox}. This inductive definition
-should help separating this proof into several steps.
-*}
-
-inductive called_via :: "(var \<Rightarrow> var ftree) \<Rightarrow> var \<Rightarrow> var \<Rightarrow> bool"
- where "y \<in> carrier (f x) \<Longrightarrow> called_via f x y"
-     | "called_via f x y \<Longrightarrow> called_via f y z \<Longrightarrow> called_via f x z"
-
-inductive
-  substitute_co_call :: "var \<Rightarrow> var \<Rightarrow> (var \<Rightarrow> var ftree) \<Rightarrow> var ftree \<Rightarrow> bool"
-where
-    "x--y\<in>(ccApprox t) \<Longrightarrow> called_via f x x' \<Longrightarrow> called_via f y y' \<Longrightarrow> substitute_co_call x' y' f t"
-
-thm substitute''.intros
-lemma ccApprox_substitute_co_call:
-  assumes "x--y\<in>(ccApprox (substitute f T t))"
-  shows   "substitute_co_call x y f t"
-proof-
-  from assms
-  obtain xs where "xs \<in> paths (substitute f T t)" and "x--y\<in>(ccFromList xs)"
-    by (auto simp add: in_ccApprox)
-  from this(1)
-  obtain xs' where "substitute'' f T xs' xs"  and "xs' \<in> paths t"  by (auto simp add: substitute_substitute'')
-  from this `x--y\<in>(ccFromList xs)`
-  show  "substitute_co_call x y f t"
-  proof(induction arbitrary: t rule: substitute''.induct[case_names Nil Cons])
-  case Nil thus ?case by simp
-  next
-  case (Cons zs f x' xs' xs T ys)
-    from `x' # xs \<in> paths t`
-    have "possible t x'" and  "xs \<in> paths (nxt t x')"
-      by (auto simp add: Cons_path)
-    
-    from this(2) and `xs' \<in> xs \<otimes> zs` and `zs \<in> paths (f x')`
-    have "xs' \<in> paths (nxt t x' \<otimes>\<otimes> f x')" by (auto simp add: paths_both)
-
-    {
-    assume "x--y\<in>(ccFromList ys)"
-    from Cons.IH[OF `xs' \<in> paths (nxt t x' \<otimes>\<otimes> f x')` this]
-    have "substitute_co_call x y (f_nxt f T x') (nxt t x' \<otimes>\<otimes> f x')".
-    
-    have ?case sorry
-    }
-    moreover
-    
-    ultimately
-    show ?case using  `x--y\<in>(ccFromList (x' # ys))`
-      apply auto
-
-    { assume "x' \<noteq> x" and "x' \<noteq> y"
-      with `x--y\<in>(ccFromList (x' # xs))`
-      have "x--y\<in>(ccFromList xs)" by simp
-      from Cons.IH[OF `xs \<in> _ ` this]
-      have "substitute_co_call x y (f_nxt f T x') (nxt t x' \<otimes>\<otimes> f x')".
-      then obtain x0 y0 where "x0--y0\<in>(ccApprox (nxt t x' \<otimes>\<otimes> f x'))"
-                          and "called_via (f_nxt f T x') x0 x"
-                          and "called_via (f_nxt f T x') y0 y" by (auto elim: substitute_co_call.cases)
-
-      from `called_via (f_nxt f T x') x0 x`
-      have "called_via f x0 x" sorry
-      from `called_via (f_nxt f T x') y0 y`
-      have "called_via f y0 y" sorry
-
-
-      from `x0--y0\<in>(ccApprox (nxt t x' \<otimes>\<otimes> f x'))`
-      have ?case
-      proof(auto simp add: ccApprox_both)
-        assume "x0--y0\<in>(ccApprox (f x'))"
-        show ?thesis   sorry
-      next
-        assume "x0--y0\<in>(ccApprox (nxt t x'))"
-        hence "x0--y0\<in>(ccApprox t)" sorry
-        moreover
-        note `called_via f x0 x`
-        moreover
-        note `called_via f y0 y`
-        ultimately
-        show ?thesis..
-     next
-       assume "x0 \<in> carrier (nxt t x')"
-       hence "x0--x' \<in>(ccApprox t)" sorry
-       moreover
-       note `called_via f x0 x`
-       moreover
-       assume "y0 \<in> carrier (f x')"
-       hence "called_via f x' y0" sorry
-       from this  `called_via f y0 y`
-       have "called_via f x' y" sorry
-       ultimately
-       show ?thesis..
-    next
-       assume "y0 \<in> carrier (nxt t x')"
-       hence "x'--y0 \<in>(ccApprox t)" sorry
-       moreover
-       assume "x0 \<in> carrier (f x')"
-       hence "called_via f x' x0" sorry
-       from this  `called_via f x0 x`
-       have "called_via f x' x" sorry
-       moreover
-       note `called_via f y0 y`
-       ultimately
-       show ?thesis..
-    qed
-    }
-    
-    show ?case
-oops
-*)
-
-(*
-lemma ccApprox_substitute_aux:
-  assumes "substitute'' f T xs ys"
-  assumes "ccFromList (prefix@xs) \<sqsubseteq> G"
-  assumes "\<And> x. x \<in> set ys \<Longrightarrow> ccApprox (f x) \<sqsubseteq> G" 
-  shows   "ccFromList (prefix@ys) \<sqsubseteq> G"
-using assms
-proof(induction f T xs ys arbitrary: prefix rule: substitute''.induct[case_names Nil Cons])
-  case Nil thus ?case by simp
-next
-  case (Cons zs f x xs' xs T ys)
-  from `ccFromList (prefix @ x # xs) \<sqsubseteq> G`
-  have  "ccFromList prefix \<sqsubseteq> G"
-    and "ccProd (set prefix) (insert x (set xs)) \<sqsubseteq> G"
-    and "ccProd {x} (set xs) \<sqsubseteq> G"
-    and "ccFromList xs \<sqsubseteq> G"
-    by (auto simp add: join_below_iff)
-
-  from Cons have "ccApprox (f x) \<sqsubseteq> G" and *: "\<And>x. x \<in> set ys \<Longrightarrow> ccApprox (f x) \<sqsubseteq> G" by auto
-  with Cons.hyps(1)
-  have "ccFromList zs \<sqsubseteq> G" by (metis below_trans ccFromList_below_ccApprox) 
-  
-  have "ccFromList ((prefix@[x])@ys) \<sqsubseteq> G"
-  proof (rule Cons.IH)
-    have "ccProd {x} (set zs) \<sqsubseteq> G" sorry
-    moreover
-    have "ccFromList zs \<sqsubseteq> G" by fact
-    moreover
-    have "ccProd (set xs) (set zs) \<sqsubseteq> G" sorry
-    moreover
-    have "ccProd (set prefix) (set zs) \<sqsubseteq> G" sorry
-    moreover
-    note `ccFromList (prefix @ x # xs) \<sqsubseteq> G`
-    ultimately
-    show "ccFromList ((prefix @ [x]) @ xs') \<sqsubseteq> G"    
-      using interleave_ccFromList[OF `xs' \<in> xs \<otimes> zs`] interleave_set[OF  `xs' \<in> xs \<otimes> zs`]
-          by (auto simp add: ccApprox_both join_below_iff ccProd_insert2[where S' = "S \<union> S'" for S S'] ccProd_insert2[where S' = "set xs" for xs])
-  next
-    fix x'
-    assume "x' \<in> set ys"
-    thus "ccApprox (f_nxt f T x x') \<sqsubseteq> G" sorry
-  qed
-  moreover
-  thm Cons
-  have "ccProd {x} (set ys) \<sqsubseteq> G" sorry
-  ultimately
-  show ?case by simp
-qed
-
-lemma ccFTree_Let:
-  assumes "isLinear \<Delta> e a"
-  shows "ccFTree (edom (ABinds \<Delta>\<cdot>(Aheap \<Delta> e\<cdot>a) \<squnion> Aexp e\<cdot>a)) (ccHeap \<Delta> e\<cdot>a) \<sqsubseteq>
-         ccFTree (edom (Aheap \<Delta> e\<cdot>a \<squnion> Aexp (Let \<Delta> e)\<cdot>a)) (ccExp (Let \<Delta> e)\<cdot>a)"
- using Aexp_Let[of \<Delta> e a]  ccExp_Let_linear[OF assms] 
- by (rule below_trans[OF ccFTree_mono1[OF edom_mono] ccFTree_mono2])
-
-lemma substitute'_valid_list:
-  assumes "xs \<in> paths (substitute f (thunks \<Delta>) t)"
-  assumes "f = env_restr (- (S \<inter> thunks \<Delta>)) (Fexp.AnalBinds \<Delta>\<cdot>(Aheap \<Delta> e\<cdot>a))" 
-  assumes "ccProd (carrier t) S \<sqsubseteq> ccBindsExtra \<Delta>\<cdot>(Aheap \<Delta> e\<cdot>a, ccHeap \<Delta> e\<cdot>a) \<squnion> ccExp e\<cdot>a"
-  shows   "valid_lists' (edom (ABinds \<Delta>\<cdot>(Aheap \<Delta> e\<cdot>a) \<squnion> Aexp e\<cdot>a)) (ccBindsExtra \<Delta>\<cdot>(Aheap \<Delta> e\<cdot>a, ccHeap \<Delta> e\<cdot>a) \<squnion> ccExp e\<cdot>a) S xs"
-using assms
-proof(induction  f "thunks \<Delta>" t xs arbitrary: S rule: substitute_induct)
-  case Nil
-  thus ?case by simp
-next
-  case (Cons f t x xs)
-
-  from `x # xs \<in> paths (substitute f (thunks \<Delta>) t)`
-  have "possible t x" and "xs \<in> paths (substitute (f_nxt f (thunks \<Delta>) x) (thunks \<Delta>) (nxt t x \<otimes>\<otimes> f x))"
-    by auto
-
-  note this(2)
-  moreover
-
-  have [simp]: "(- {x} \<inter> (- S \<union> - thunks \<Delta>)) = (- insert x (S \<inter> thunks \<Delta>))" by auto
-    
-  from  Cons.prems(2)
-  have "f_nxt f (thunks \<Delta>) x = env_restr (-(insert x S \<inter> thunks \<Delta>)) (ExpAnalysis.AnalBinds Fexp \<Delta>\<cdot>(Aheap \<Delta> e\<cdot>a))"
-    by (cases "x \<in> thunks \<Delta>")
-       (auto simp add: f_nxt_def env_delete_def[symmetric] empty_is_bottom env_delete_restr)
-  moreover
-  from below_trans[OF ccProd_mono1[OF carrier_nxt_subset] `ccProd (carrier t) _ \<sqsubseteq> _`]
-  have "ccProd (carrier (nxt t x \<otimes>\<otimes> f x)) (insert x S) \<sqsubseteq> ccBindsExtra \<Delta>\<cdot>(Aheap \<Delta> e\<cdot>a, ccHeap \<Delta> e\<cdot>a) \<squnion> ccExp e\<cdot>a" 
-    apply (auto simp add: join_below_iff ccProd_insert2[where S' = S])
-    thm ccProd_mono1[OF carrier_nxt_subset]
-    sor ry
-  ultimately
-  have IH: "valid_lists' (edom (ABinds \<Delta>\<cdot>(Aheap \<Delta> e\<cdot>a) \<squnion> Aexp e\<cdot>a)) (ccBindsExtra \<Delta>\<cdot>(Aheap \<Delta> e\<cdot>a, ccHeap \<Delta> e\<cdot>a) \<squnion> ccExp e\<cdot>a) (insert x S) xs"  
-    by (rule Cons.hyps)
-
-  have "x \<in> carrier t" by (metis `possible t x` carrier_possible)
-  hence "ccProd {x} S \<sqsubseteq> ccProd (carrier t) S" by (auto intro: ccProd_mono1)
-  with `ccProd (carrier t) _ \<sqsubseteq> _`
-  have "S \<subseteq> ccNeighbors {x} (ccBindsExtra \<Delta>\<cdot>(Aheap \<Delta> e\<cdot>a, ccHeap \<Delta> e\<cdot>a) \<squnion> ccExp e\<cdot>a)"
-    unfolding subset_ccNeighbors
-    by (rule below_trans[rotated])
-  moreover
-  note IH
-  moreover
-  have "x \<in> edom (ABinds \<Delta>\<cdot>(Aheap \<Delta> e\<cdot>a) \<squnion> Aexp e\<cdot>a)" sorry
-  ultimately
-  show ?case..
-qed
-*)
-
-lemma in_carrier_fup[simp]:
-  "x' \<in> carrier (fup\<cdot>f\<cdot>u) \<longleftrightarrow> (\<exists> u'. u = up\<cdot>u' \<and> x' \<in> carrier (f\<cdot>u'))"
-  by (cases u) auto
-
-lemma carrier_AnalBinds_below:
-  "carrier ((Fexp.AnalBinds  \<Delta>\<cdot>(Aheap \<Delta> e\<cdot>a)) x) \<subseteq> edom ((ABinds \<Delta>)\<cdot>(Aheap \<Delta> e\<cdot>a))"
-by (auto simp add: Fexp.AnalBinds_lookup Fexp_def split: option.splits 
-         elim!: set_mp[OF edom_mono[OF monofun_cfun_fun[OF ABind_below_ABinds]]])
 
 sublocale FutureAnalysisCardinalityHeap Fexp Aexp Aheap Fheap
 proof default
@@ -1582,5 +339,164 @@ next
 
 qed
 end
+
+(* TODO: Unused stuff from here, mostly about singles. Might be useful later. *)
+
+
+lemma paths_singles: "xs \<in> paths (singles S) \<longleftrightarrow> (\<forall>x \<in> S. one_call_in_path x xs)"
+  by transfer (auto simp add: one_call_in_path_filter_conv)
+
+lemma paths_singles': "xs \<in> paths (singles S) \<longleftrightarrow> (\<forall>x \<in> (set xs \<inter> S). one_call_in_path x xs)"
+  apply transfer
+  apply (auto simp add: one_call_in_path_filter_conv)
+  apply (erule_tac x = x in ballE)
+  apply auto
+  by (metis (poly_guards_query) filter_empty_conv le0 length_0_conv)
+
+lemma both_below_singles1:
+  assumes "t \<sqsubseteq> singles S"
+  assumes "carrier t' \<inter> S = {}"
+  shows "t \<otimes>\<otimes> t' \<sqsubseteq> singles S"
+proof (rule ftree_belowI)
+  fix xs
+  assume "xs \<in> paths (t \<otimes>\<otimes> t')"
+  then obtain ys zs where "ys \<in> paths t" and "zs \<in> paths t'" and "xs \<in> ys \<otimes> zs" by (auto simp add: paths_both)
+  with assms 
+  have "ys \<in> paths (singles S)" and "set zs \<inter> S = {}"
+    by (metis below_ftree.rep_eq contra_subsetD paths.rep_eq, auto simp add: Union_paths_carrier[symmetric])
+  with `xs \<in> ys \<otimes> zs`
+  show "xs \<in> paths (singles S)"
+    by (induction) (auto simp add: paths_singles no_call_in_path_set_conv interleave_set dest: more_than_one_setD split: if_splits)
+qed
+
+
+lemma paths_ftree_restr_singles: "xs \<in> paths (ftree_restr S' (singles S)) \<longleftrightarrow> set xs \<subseteq> S' \<and> (\<forall>x \<in> S. one_call_in_path x xs)"
+proof
+  show "xs \<in> paths (ftree_restr S' (singles S)) \<Longrightarrow>  set xs \<subseteq> S' \<and> (\<forall>x \<in> S. one_call_in_path x xs)"
+    by (auto simp add: filter_paths_conv_free_restr[symmetric] paths_singles)
+next
+  assume *: "set xs \<subseteq> S' \<and> (\<forall>x\<in>S. one_call_in_path x xs)"
+  hence "set xs \<subseteq> S'" by auto
+  hence [simp]: "filter (\<lambda> x'. x' \<in> S') xs = xs" by (auto simp add: filter_id_conv)
+  
+  from *
+  have "xs \<in> paths (singles S)"
+     by (auto simp add: paths_singles')
+  hence "filter (\<lambda> x'. x' \<in> S') xs \<in> filter (\<lambda>x'. x' \<in> S') ` paths (singles S)"
+    by (rule imageI)
+  thus "xs \<in> paths (ftree_restr S' (singles S))"
+    by (auto simp add: filter_paths_conv_free_restr[symmetric] )
+qed
+
+
+
+(* TODO: unused *)
+lemma substitute_not_carrier:
+  assumes "x \<notin> carrier t"
+  assumes "\<And> x'. x \<notin> carrier (f x')"
+  shows "x \<notin>  carrier (substitute f T t)"
+proof-
+  have "ftree_restr ({x}) (substitute f T t) = ftree_restr ({x}) t"
+  proof(rule ftree_rest_substitute)
+    fix x'
+    from `x \<notin> carrier (f x')`
+    show "carrier (f x') \<inter> {x} = {}" by auto
+  qed
+  hence "x \<notin> carrier (ftree_restr ({x}) (substitute f T t)) \<longleftrightarrow> x \<notin> carrier (ftree_restr ({x}) t)" by metis
+  with assms(1)
+  show ?thesis by simp
+qed
+
+(* TODO: unused *)
+lemma substitute_below_singlesI:
+  assumes "t \<sqsubseteq> singles S"
+  assumes "\<And> x. carrier (f x) \<inter> S = {}"
+  shows "substitute f T t \<sqsubseteq> singles S"
+proof(rule ftree_belowI)
+  fix xs
+  assume "xs \<in> paths (substitute f T t)"
+  thus "xs \<in> paths (singles S)"
+  using assms
+  proof(induction f T t xs arbitrary: S rule: substitute_induct)
+    case Nil
+    thus ?case by simp
+  next
+    case (Cons f T t x xs)
+
+    from `x#xs \<in> _`
+    have xs: "xs \<in> paths (substitute (f_nxt f T x) T (nxt t x \<otimes>\<otimes> f x))" by auto
+    moreover
+
+    from `t \<sqsubseteq> singles S`
+    have "nxt t x \<sqsubseteq> singles S" 
+      by (metis "FTree-HOLCF.nxt_mono" below_trans nxt_singles_below_singles)
+    from this `carrier (f x) \<inter> S = {}`
+    have "nxt t x \<otimes>\<otimes> f x \<sqsubseteq> singles S"
+      by (rule both_below_singles1)
+    moreover
+    { fix x'
+      from  `carrier (f x') \<inter> S = {}`
+      have "carrier (f_nxt f T x x') \<inter> S = {}"
+        by (auto simp add: f_nxt_def)
+    }
+    ultimately
+    have IH: "xs \<in> paths (singles S)"
+      by (rule Cons.IH) 
+  
+  show ?case
+    proof(cases "x \<in> S")
+      case True
+      with `carrier (f x) \<inter> S = {}`
+      have "x \<notin> carrier (f x)" by auto
+      moreover
+      from `t \<sqsubseteq> singles S`
+      have "nxt t x \<sqsubseteq> nxt (singles S) x" by (rule nxt_mono)
+      hence "carrier (nxt t x) \<subseteq> carrier (nxt (singles S) x)" by (rule carrier_mono)
+      from set_mp[OF this] True
+      have "x \<notin> carrier (nxt t x)" by auto
+      ultimately
+      have "x \<notin> carrier (nxt t x \<otimes>\<otimes> f x)" by simp
+      hence "x \<notin> carrier (substitute (f_nxt f T x) T (nxt t x \<otimes>\<otimes> f x))"
+      proof(rule substitute_not_carrier)
+        fix x'  
+        from `carrier (f x') \<inter> S = {}` `x \<in> S`
+        show "x \<notin> carrier (f_nxt f T x x')" by (auto simp add: f_nxt_def)
+      qed
+      with xs
+      have "x \<notin> set xs" by (auto simp add: Union_paths_carrier[symmetric])
+      with IH
+      have "xs \<in> paths (without x (singles S))" by (rule paths_withoutI)
+      thus ?thesis using True by (simp add: Cons_path)
+    next
+      case False
+      with IH
+      show ?thesis by (simp add: Cons_path)
+    qed
+  qed
+qed
+
+(* TODO: Unused. Remove? *)
+lemma multi_calls_ccFTree:
+  assumes "xs \<in> paths (ccFTree S G)"
+  assumes "\<not> one_call_in_path x xs"
+  shows "x \<in> S" and "x \<in> ccManyCalls G"
+proof-
+  from assms(1) have "xs \<in> valid_lists S G" by simp 
+
+  have "x \<in> set xs" by (metis assms(2) filter_True one_call_in_path_filter)
+  with `xs \<in> valid_lists S G`
+  show "x \<in> S" by (metis  subsetCE valid_lists_subset)
+
+  show "x \<in> ccManyCalls G"
+  proof(rule ccontr)
+    assume "x \<notin> ccManyCalls G"
+    with `xs \<in> valid_lists S G` 
+    have "one_call_in_path x xs"
+    by (induction rule: valid_lists.induct) (auto simp add: no_call_in_path_set_conv)
+    with assms(2)
+    show False..
+  qed
+qed
+
 
 end
