Launchbury/RedsImprovesArityAnalysis.thy
@@ -99,13 +99,13 @@ case (Variable \<Gamma> x e L \<Delta> z ae n)
     finally have "Afix \<Delta>\<cdot>(Aexp' z\<cdot>(n \<squnion> aeL x) \<squnion> ae) f|` ?S \<sqsubseteq> Afix (delete x \<Gamma>)\<cdot>(Aexp' e\<cdot>(n \<squnion> aeR x) \<squnion> ae) f|` ?S" by this simp_all
     thus ?case by simp
   qed simp_all
-  also have "\<dots> \<sqsubseteq> (\<mu> ae'. Afix ((x,e)#delete x \<Gamma>) \<cdot> (AE_singleton x \<cdot> (n \<squnion> ae' x) \<squnion> ae))  f|` ?S"
+  also have "\<dots> \<sqsubseteq> (\<mu> ae'. Afix ((x,e)#delete x \<Gamma>) \<cdot> (esing x \<cdot> (n \<squnion> ae' x) \<squnion> ae))  f|` ?S"
     apply (rule env_restr_mono)
     apply (rule monofun_cfun_arg)
     apply (rule cfun_belowI, simp)
     apply (rule Afix_e_to_heap[simplified])
     done
-  also have "\<dots> = Afix ((x,e)#delete x \<Gamma>) \<cdot> (AE_singleton x\<cdot>n \<squnion> ae)  f|` ?S" by (rule arg_cong[OF Afix_repeat_singleton])
+  also have "\<dots> = Afix ((x,e)#delete x \<Gamma>) \<cdot> (esing x\<cdot>n \<squnion> ae)  f|` ?S" by (rule arg_cong[OF Afix_repeat_singleton])
   also have "\<dots> \<sqsubseteq> Afix ((x,e)#delete x \<Gamma>) \<cdot> (Aexp' (Var x) \<cdot> n \<squnion> ae)  f|` ?S" by (intro Aexp'_Var monofun_cfun env_restr_mono join_mono below_refl)
   also have "\<dots> = Afix \<Gamma> \<cdot> (Aexp' (Var x)\<cdot>n \<squnion> ae) f|` ?S" by (rule arg_cong[OF Afix_reorder[OF reorder]])
   finally show "Afix ((x, z) # \<Delta>)\<cdot>(Aexp' z\<cdot>n \<squnion> ae) f|` ?S \<sqsubseteq> Afix \<Gamma>\<cdot>(Aexp' (Var x)\<cdot>n \<squnion> ae) f|` ?S"
@@ -114,7 +114,7 @@ next
 case (Application y \<Gamma> e x L \<Delta> \<Theta> z e' ae n)
   note prem1 =  `edom ae \<subseteq> set L`
   hence prem2: "edom ae \<subseteq> set (x#L)" by auto
-  hence prem3: "edom (AE_singleton x\<cdot>(up\<cdot>0) \<squnion> ae) \<subseteq> set (x#L)" by auto
+  hence prem3: "edom (esing x\<cdot>(up\<cdot>0) \<squnion> ae) \<subseteq> set (x#L)" by auto
 
   have subset1: " (- (domA \<Theta> - domA \<Gamma>)) \<subseteq> (- (domA \<Theta> - domA \<Delta>))"
     and subset2: "(- (domA \<Theta> - domA \<Gamma>)) \<subseteq> (- (domA \<Delta> - domA \<Gamma>))"
@@ -132,13 +132,13 @@ case (Application y \<Gamma> e x L \<Delta> \<Theta> z e' ae n)
     note IH1 = env_restr_below_subset[OF subset2 Application(3)[OF prem3, where n = "inc\<^sub>\<bottom>\<cdot>n"], unfolded up Aexp'_simps inc_bot_simps] 
     note IH2 = env_restr_below_subset[OF subset1 Application(5)[OF prem1, where n = n], unfolded up Aexp'_simps]
     have "Afix \<Theta>\<cdot>(Aexp z\<cdot>n' \<squnion> ae)  f|` ?S  \<sqsubseteq> Afix \<Delta>\<cdot>(Aexp e'[y::=x]\<cdot>n' \<squnion> ae)  f|` ?S" by (rule IH2)
-    also have "\<dots> \<sqsubseteq> Afix \<Delta>\<cdot>(env_delete y (Aexp e'\<cdot>n') \<squnion>  AE_singleton x \<cdot> (up\<cdot>0) \<squnion> ae)  f|` ?S"
+    also have "\<dots> \<sqsubseteq> Afix \<Delta>\<cdot>(env_delete y (Aexp e'\<cdot>n') \<squnion>  esing x \<cdot> (up\<cdot>0) \<squnion> ae)  f|` ?S"
       by (intro monofun_cfun_arg monofun_cfun_fun env_restr_mono Aexp_subst join_mono below_refl)  
-    also have "\<dots> = Afix \<Delta>\<cdot>(env_delete y (Aexp e'\<cdot>(pred\<cdot>(inc\<cdot>n'))) \<squnion> (AE_singleton x \<cdot> (up\<cdot>0) \<squnion> ae))  f|` ?S" by simp
-    also have "\<dots> \<sqsubseteq> Afix \<Delta>\<cdot>(Aexp (Lam [y]. e')\<cdot>(inc\<cdot>n') \<squnion> (AE_singleton x \<cdot> (up\<cdot>0) \<squnion> ae))  f|` ?S"
+    also have "\<dots> = Afix \<Delta>\<cdot>(env_delete y (Aexp e'\<cdot>(pred\<cdot>(inc\<cdot>n'))) \<squnion> (esing x \<cdot> (up\<cdot>0) \<squnion> ae))  f|` ?S" by simp
+    also have "\<dots> \<sqsubseteq> Afix \<Delta>\<cdot>(Aexp (Lam [y]. e')\<cdot>(inc\<cdot>n') \<squnion> (esing x \<cdot> (up\<cdot>0) \<squnion> ae))  f|` ?S"
       by (intro monofun_cfun_arg monofun_cfun_fun env_restr_mono Aexp_Lam join_mono below_refl)  
-    also have "\<dots> \<sqsubseteq> Afix \<Gamma>\<cdot>(Aexp e\<cdot>(inc\<cdot>n') \<squnion> (AE_singleton x\<cdot>(up\<cdot>0) \<squnion> ae)) f|` ?S" by (rule IH1)
-    also have "\<dots> = Afix \<Gamma>\<cdot>(Aexp e\<cdot>(inc\<cdot>n') \<squnion> AE_singleton x\<cdot>(up\<cdot>0) \<squnion> ae)  f|` ?S" by simp
+    also have "\<dots> \<sqsubseteq> Afix \<Gamma>\<cdot>(Aexp e\<cdot>(inc\<cdot>n') \<squnion> (esing x\<cdot>(up\<cdot>0) \<squnion> ae)) f|` ?S" by (rule IH1)
+    also have "\<dots> = Afix \<Gamma>\<cdot>(Aexp e\<cdot>(inc\<cdot>n') \<squnion> esing x\<cdot>(up\<cdot>0) \<squnion> ae)  f|` ?S" by simp
     also have "\<dots> \<sqsubseteq> Afix \<Gamma>\<cdot>(Aexp (App e x)\<cdot>n' \<squnion> ae)  f|` ?S" 
       by (intro monofun_cfun_arg monofun_cfun_fun env_restr_mono Aexp_App join_mono below_refl)  
     finally
